coq/cclc3/clc_uniq.v
@@ -6,25 +6,155 @@ Set Implicit Arguments.
 Unset Strict Implicit.
 Unset Printing Implicit Defensive.
 
+Inductive head_sim : term -> term -> Prop :=
+| head_sim_var x : head_sim (Var x) (Var x)
+| head_sim_sort s : head_sim (Sort s) (Sort s)
+| head_sim_pi A1 A2 B1 B2 s t :
+  head_sim A1 A2 ->
+  head_sim B1 B2 ->
+  head_sim (Pi A1 B1 s t) (Pi A2 B2 s t)
+| head_sim_lam A m s t : head_sim (Lam A m s t) (Lam A m s t)
+| head_sim_app m n : head_sim (App m n) (App m n)
+| head_sim_fix A m : head_sim (Fix A m) (Fix A m)
+| head_sim_unit : head_sim (Unit) (Unit)
+| head_sim_it : head_sim (It) (It)
+| head_sim_either : head_sim (Either) (Either)
+| head_sim_left : head_sim (Left) (Left)
+| head_sim_right : head_sim (Right) (Right)
+| head_sim_sigma A1 A2 B1 B2 s1 s2 r1 r2 t1 t2 :
+  head_sim (Sigma A1 B1 s1 r1 t1) (Sigma A2 B2 s2 r2 t2)
+| head_sim_pair m n t : head_sim (Pair m n t) (Pair m n t)
+| head_sim_case A m n1 n2 : head_sim (Case A m n1 n2) (Case A m n1 n2)
+| head_sim_letin1 A m n : head_sim (LetIn1 A m n) (LetIn1 A m n)
+| head_sim_letin2 A m n : head_sim (LetIn2 A m n) (LetIn2 A m n)
+| head_sim_main : head_sim (Main) (Main)
+| head_sim_proto : head_sim (Proto) (Proto)
+| head_sim_stop r : head_sim (Stop r) (Stop r)
+| head_sim_act r A B s : head_sim (Act r A B s) (Act r A B s)
+| head_sim_ch r A : head_sim (Ch r A) (Ch r A)
+| head_sim_fork m n : head_sim (Fork m n) (Fork m n)
+| head_sim_recv ch : head_sim (Recv ch) (Recv ch)
+| head_sim_send ch : head_sim (Send ch) (Send ch)
+| head_sim_close ch : head_sim (Close ch) (Close ch)
+| head_sim_wait ch : head_sim (Wait ch) (Wait ch).
+
+Inductive sim (m n : term) : Prop :=
+| Sim x y : m === x -> head_sim x y -> y === n -> sim m n.
+
+Lemma head_sim_refl m : head_sim m m.
+Proof with eauto using head_sim. elim: m... Qed.
+Hint Resolve head_sim_refl.
+
+Lemma head_sim_subst m1 m2 σ : head_sim m1 m2 -> head_sim m1.[σ] m2.[σ].
+Proof with eauto using head_sim.
+  move=>hs. elim: hs σ=>{m1 m2}...
+Qed.
+
+Lemma sim_refl m : sim m m.
+Proof with eauto. econstructor... Qed.
+Hint Resolve sim_refl.
+
+Lemma sim_transL x y z : sim x y -> y === z -> sim x z.
+Proof with eauto.
+  move=>sm eq. inv sm.
+  econstructor...
+  apply: conv_trans...
+Qed.
+
+Lemma sim_transR x y z : sim x y -> z === x -> sim z y.
+Proof with eauto using head_sim.
+  move=>sm eq. inv sm.
+  econstructor.
+  apply: conv_trans...
+  apply: H0.
+  apply: H1.
+Qed.
+
+Lemma sim_subst x y σ : sim x y -> sim x.[σ] y.[σ].
+Proof with eauto.
+  move=>sm. inv sm.
+  econstructor.
+  apply: conv_subst...
+  apply: head_sim_subst...
+  apply: conv_subst...
+Qed.
+
+Lemma sim_sort s t : sim (Sort s) (Sort t) -> s = t.
+Proof with eauto.
+  move e1:(Sort s)=>m.
+  move e2:(Sort t)=>n sm.
+  inv sm.
+  elim: H0 s t H H1=>//{x y}.
+  all: try solve[intros; exfalso; solve_conv].
+  { move=>s r t/sort_inj->/sort_inj->//. }
+  { move=>m n s t eq1 eq2.
+    have/sort_inj//:=conv_trans _ eq1 eq2. }
+  { move=>A m s t eq1 eq2.
+    have/sort_inj//:=conv_trans _ eq1 eq2. }
+  { move=>A m n1 n2 s t eq1 eq2.
+    have/sort_inj//:=conv_trans _ eq1 eq2. }
+  { move=>A m n s t eq1 eq2.
+    have/sort_inj//:=conv_trans _ eq1 eq2. }
+  { move=>A m n s t eq1 eq2.
+    have/sort_inj//:=conv_trans _ eq1 eq2. }
+Qed.
+
+Lemma sim_pi_inj A1 A2 B1 B2 s1 s2 t1 t2 :
+  sim (Pi A1 B1 s1 t1) (Pi A2 B2 s2 t2) ->
+  sim A1 A2 /\ sim B1 B2 /\ s1 = s2 /\ t1 = t2.
+Proof with eauto.
+  move=>sm. inv sm.
+  elim: H0 A1 A2 B1 B2 s1 s2 t1 t2 H H1=>{x y}.
+  all: try solve[intros; exfalso; solve_conv].
+  { move=>A1 A2 B1 B2 s t hA ihA hB ihB A0 A3 B0 B3 s1 s2 t1 t2
+      /pi_inj[eqA1[eqB1[e1 e2]]]/pi_inj[eqA2[eqB2[e3 e4]]]; subst.
+    repeat split.
+    econstructor...
+    econstructor... }
+  { move=>m n A1 A2 B1 B2 s1 s2 t1 t2 eq1 eq2.
+    have/pi_inj[eqA[eqB[->->]]]:=conv_trans _ eq1 eq2.
+    repeat split.
+    econstructor...
+    econstructor... }
+  { move=>A m A1 A2 B1 B2 s1 s2 t1 t2 eq1 eq2.
+    have/pi_inj[eqA[eqB[->->]]]:=conv_trans _ eq1 eq2.
+    repeat split.
+    econstructor...
+    econstructor... }
+  { move=>A m n1 n2 A1 A2 B1 B2 s1 s2 t1 t2 eq1 eq2.
+    have/pi_inj[eqA[eqB[->->]]]:=conv_trans _ eq1 eq2.
+    repeat split.
+    econstructor...
+    econstructor... }
+  { move=>A m n A1 A2 B1 B2 s1 s2 t1 t2 eq1 eq2.
+    have/pi_inj[eqA[eqB[->->]]]:=conv_trans _ eq1 eq2.
+    repeat split.
+    econstructor...
+    econstructor... }
+  { move=>A m n A1 A2 B1 B2 s1 s2 t1 t2 eq1 eq2.
+    have/pi_inj[eqA[eqB[->->]]]:=conv_trans _ eq1 eq2.
+    repeat split.
+    econstructor...
+    econstructor... }
+Qed.
+
 Lemma clc_sort_uniq Γ s A :
-  Γ ⊢ Sort s : A -> Sort U === A.
+  Γ ⊢ Sort s : A -> sim (Sort U) A.
 Proof with eauto.
   move e:(Sort s)=>n ty. elim: ty s e=>//{Γ n A}.
   move=>Γ A B m s eq tym ihm tyB ihB t e; subst.
-  apply: conv_trans.
-  apply: ihm...
-  exact: eq.
+  have eq':=ihm _ erefl.
+  apply: sim_transL...
 Qed.
 
 Lemma clc_pi_uniq Γ A B s t C :
-  Γ ⊢ Pi A B s t : C -> Sort t === C.
-Proof with eauto.
+  Γ ⊢ Pi A B s t : C -> sim (Sort t) C.
+Proof with eauto using head_sim.
   move e:(Pi A B s t)=>n ty. elim: ty A B s t e=>//{Γ n C}.
   move=>Γ A B s r t k tyA ihA tyB ihB A0 B0 s0 t0[e1 e2 e3->]//.
   move=>Γ A B m s eq tym ihm tyB ihB A0 B0 s0 t e; subst.
-  apply: conv_trans.
-  apply: ihm...
-  exact: eq.
+  have eq':=ihm _ _ _ _ erefl.
+  apply: sim_transL...
 Qed.
 
 Lemma clc_has_subset Γ Γ1 Γ2 G1 G2 A B x s t :
@@ -53,147 +183,254 @@ Proof with eauto.
   { inv hs2. rewrite (ih _ _ H1)... }
 Qed.
 
-Lemma clc_var_uniq Γ A B x s :
-  Γ ⊢ Var x : B -> has Γ x s A -> A === B.
-Proof with eauto.
-  move e:(Var x)=>n ty. elim: ty A x s e=>//{Γ n B}.
-  move=>Γ x A s hs1 A0 x0 s0[e]hs2; subst.
-  { rewrite (clc_has_uniq hs1 hs2)... }
-  move=>Γ A B m s eq tym ihm tyB ihB A0 x s0 e hs; subst.
-  { apply: conv_trans.
-    apply: ihm...
-    exact: eq. }
-Qed.
-
 Lemma clc_lam_uniq Γ A B C m s t :
-  Γ ⊢ Lam A m s t : C -> (forall C, A :{s} Γ ⊢ m : C -> B === C) -> Pi A B s t === C.
+  Γ ⊢ Lam A m s t : C -> (forall C, A :{s} Γ ⊢ m : C -> sim B C) -> sim (Pi A B s t) C.
 Proof with eauto.
   move e:(Lam A m s t)=>n ty. elim: ty A B m s t e=>//{Γ n C}.
   move=>Γ A B m s t k tyP ihP tym ihm A0 B0 m0 s0 t0[e1 e2 e3 e4]h; subst.
-  { have eq:=h _ tym.
+  { have eq':=h _ tym. inv eq'.
+    econstructor.
+    apply: conv_pi.
+    eauto.
+    apply: H.
+    constructor.
+    eauto.
+    apply: H0.
     apply: conv_pi... }
   move=>Γ A B m s eq tym ihm tyB ihB A0 B0 m0 s0 t e h; subst.
-  { apply: conv_trans.
-    apply: ihm...
-    exact: eq. }
+  { have eq':=ihm _ _ _ _ _ erefl h.
+    apply: sim_transL... }
 Qed.
 
 Lemma clc_app_uniq Γ A B C m n s t :
   Γ ⊢ App m n : C ->
-  (forall C Γ1 Γ2, Γ1 ∘ Γ2 => Γ -> Γ1 ⊢ m : C -> Pi A B s t === C) -> B.[n/] === C.
+  (forall C Γ1 Γ2, Γ1 ∘ Γ2 => Γ -> Γ1 ⊢ m : C -> sim (Pi A B s t) C) -> sim B.[n/] C.
 Proof with eauto.
   move e:(App m n)=>x ty. elim: ty A B m n s t e=>//{Γ x C}.
   move=>Γ1 Γ2 Γ A B m n s t k mrg tym ihm tyn ihn
      A0 B0 m0 n0 s0 t0[e1 e2]h; subst.
-  { have/pi_inj[_[eq _]]:=h _ _ _ mrg tym.
-    apply: conv_subst... }
+  { have/sim_pi_inj[_[eq' _]]:=h _ _ _ mrg tym.
+    apply: sim_subst... }
   move=>Γ A B m s eq tym ihm tyB ihB A0 B0 m0 n s0 t e h; subst.
-  { apply: conv_trans.
-    apply: ihm...
-    exact: eq. }
+  { have eq':=ihm _ _ _ _ _ _ erefl h.
+    apply: sim_transL... }
 Qed.
 
-Lemma clc_fix_uniq Γ A B m : Γ ⊢ Fix A m : B -> A === B.
+Lemma clc_fix_uniq Γ A B m : Γ ⊢ Fix A m : B -> sim A B.
 Proof with eauto.
   move e:(Fix A m)=>n ty. elim: ty A m e=>//{Γ B n}.
   move=>Γ A m k tyA ihA tym ihm A0 m0[e1 e2]; subst...
   move=>Γ A B m s eq tym ihm tyB ihB A0 m0 e; subst.
-  { apply: conv_trans.
-    apply: ihm...
-    exact: eq. }
+  { have eq':=ihm _ _ erefl.
+    apply: sim_transL... }
 Qed.
 
-Lemma clc_unit_uniq Γ A : Γ ⊢ Unit : A -> Sort U === A.
+Lemma clc_unit_uniq Γ A : Γ ⊢ Unit : A -> sim (Sort U) A.
 Proof with eauto.
   move e:(Unit)=>m ty. elim: ty e=>//{Γ m A}.
   move=>Γ A B m s eq tym ihm tyB ihB e; subst.
-  { apply: conv_trans.
-    apply: ihm...
-    exact: eq. }
+  { have eq':=ihm erefl.
+    apply: sim_transL... }
 Qed.
 
-Lemma clc_it_uniq Γ A : Γ ⊢ It : A -> Unit === A.
+Lemma clc_it_uniq Γ A : Γ ⊢ It : A -> sim Unit A.
 Proof with eauto.
   move e:(It)=>m ty. elim: ty e=>//{Γ m A}.
   move=>Γ A B m s eq tym ihm tyB ihB e; subst.
-  { apply: conv_trans.
-    apply: ihm...
-    exact: eq. }
+  { have eq':=ihm erefl.
+    apply: sim_transL... }
 Qed.
 
-Lemma clc_either_uniq Γ A : Γ ⊢ Either : A -> Sort U === A.
+Lemma clc_either_uniq Γ A : Γ ⊢ Either : A -> sim (Sort U) A.
 Proof with eauto.
   move e:(Either)=>m ty. elim: ty e=>//{Γ m A}.
   move=>Γ A B m s eq tym ihm tyB ihB e; subst.
-  { apply: conv_trans.
-    apply: ihm...
-    exact: eq. }
+  { have eq':=ihm erefl.
+    apply: sim_transL... }
 Qed.
 
-Lemma clc_left_uniq Γ A : Γ ⊢ Left : A -> Either === A.
+Lemma clc_left_uniq Γ A : Γ ⊢ Left : A -> sim Either A.
 Proof with eauto.
   move e:(Left)=>m ty. elim: ty e=>//{Γ m A}.
   move=>Γ A B m s eq tym ihm tyB ihB e; subst.
-  { apply: conv_trans.
-    apply: ihm...
-    exact: eq. }
+  { have eq':=ihm erefl.
+    apply: sim_transL... }
 Qed.
 
-Lemma clc_right_uniq Γ A : Γ ⊢ Right : A -> Either === A.
+Lemma clc_right_uniq Γ A : Γ ⊢ Right : A -> sim Either A.
 Proof with eauto.
   move e:(Right)=>m ty. elim: ty e=>//{Γ m A}.
   move=>Γ A B m s eq tym ihm tyB ihB e; subst.
-  { apply: conv_trans.
-    apply: ihm...
-    exact: eq. }
+  { have eq':=ihm erefl.
+    apply: sim_transL... }
 Qed.
 
 Lemma clc_sigma_uniq Γ A B C s r t :
-  Γ ⊢ Sigma A B s r t : C -> Sort t === C.
+  Γ ⊢ Sigma A B s r t : C -> sim (Sort t) C.
 Proof with eauto.
   move e:(Sigma A B s r t)=>m ty. elim: ty A B s r t e=>//{Γ m C}.
   move=>Γ A B s r t leq k tyA ihA tyB ihB A0 B0 s0 r0 t0[e1 e2 e3 e4 e5]; subst...
   move=>Γ A B m s eq tym ihm tyB ihB A0 B0 s0 r t e; subst.
-  { apply: conv_trans.
-    apply: ihm...
-    exact: eq. }
+  { have eq':=ihm _ _ _ _ _ erefl.
+    apply: sim_transL... }
 Qed.
 
 Lemma clc_pair_uniq Γ A B C m n s r t :
   Γ ⊢ Pair m n t : C ->
-  [Γ] ⊢ A : Sort s ->
-  [A :{s} Γ] ⊢ B : Sort r ->
   (forall Γ1 Γ2 G1 G2 X Y,
       Γ1 ⊢ m : X -> Γ1 ∘ G1 => Γ ->
-      Γ2 ⊢ n : Y -> G2 ∘ Γ2 => Γ -> A === X /\ B.[m/] === Y) -> Sigma A B s r t === C.
+      Γ2 ⊢ n : Y -> G2 ∘ Γ2 => Γ -> sim A X /\ sim B.[m/] Y) -> sim (Sigma A B s r t) C.
 Proof with eauto.
-  move e:(Pair m n t)=>x ty. elim: ty m n A B s r t e=>//{Γ x C}.
-  move=>Γ1 Γ2 Γ A B m n s r t k1 k2 mrg1 tyS _ tym _ tyn _ m0 n0 A0 B0
-    s0 r0 t0[e1 e2 e3]tyA0 tyB0 h; subst.
+  move e:(Pair m n t)=>x ty. elim: ty A B m n t s r e=>//{Γ C x}.
+  { move=>Γ1 Γ2 Γ A B m n s r t k1 k2 mrg tyS _ tym _ tyn _ A0 B0 m0 n0
+      t0 s0 r0[e1 e2 e3]h; subst.
+    econstructor. eauto.
+    constructor. eauto. }
+  { move=>Γ A B m s eq tym ihm tyB _ A0 B0 m0 n t s0 r e h; subst.
+    have eq':=ihm _ _ _ _ _ s0 r erefl h.
+    apply: sim_transL... }
+Qed.
 
-(* Lemma clc_app_uniq Γ A B C m n s t : *)
-(*   Γ ⊢ App m n : C -> *)
-(*   (forall C Γ1 Γ2, Γ1 ∘ Γ2 => Γ -> Γ1 ⊢ m : C -> Pi A B s t === C) -> B.[n/] === C. *)
+Lemma clc_case_uniq Γ m n1 n2 A B :
+  Γ ⊢ Case A m n1 n2 : B -> sim A.[m/] B.
+Proof with eauto.
+  move e:(Case A m n1 n2)=>x ty. elim: ty A m n1 n2 e=>//{Γ B x}.
+  { move=>Γ1 Γ2 Γ m n1 n2 A s t k mrg tym _ tyA _ tyn1 _ tyn2 _
+      A0 m0 n0 n3[e1 e2 e3 e4]; subst.
+    apply: sim_refl. }
+  { move=>Γ A B m s eq tym ihm tyB _ A0 m0 n1 n2 e; subst.
+    have eq':=ihm _ _ _ _ erefl.
+    apply: sim_transL... }
+Qed.
 
-(*   ihm : ∀ (Γ2 G1 G2 Γ : context term) (B : term), Γ2 ⊢ m : B → Γ1 ∘ G1 => Γ → Γ2 ∘ G2 => Γ → A === B *)
-(*   tyn : Γ2 ⊢ n : B.[m/] *)
-(*   ihn : ∀ (Γ3 G1 G2 Γ : context term) (B0 : term), Γ3 ⊢ n : B0 → Γ2 ∘ G1 => Γ → Γ3 ∘ G2 => Γ → B.[m/] === B0 *)
-(*   Γ0, G1, G2, Γ3 : context term *)
-(*   B0 : term *)
-(*   tyP : Γ0 ⊢ Pair m n t : B0 *)
+Lemma clc_letin1_uniq Γ m n A B :
+  Γ ⊢ LetIn1 A m n : B -> sim A.[m/] B.
+Proof with eauto.
+  move e:(LetIn1 A m n)=>x ty. elim: ty A m n e=>//{Γ B x}.
+  { move=>Γ1 Γ2 Γ m n A s t k mrg tym _ tyA _ tyn _
+      A0 m0 n0[e1 e2 e3]; subst.
+    apply: sim_refl. }
+  { move=>Γ A B m s k tym ihm tyB _ A0 m0 n e; subst.
+    have eq':=ihm _ _ _ erefl.
+    apply: sim_transL... }
+Qed.
+    
+Lemma clc_letin2_uniq Γ m n A B :
+  Γ ⊢ LetIn2 A m n : B -> sim A.[m/] B.
+Proof with eauto.
+  move e:(LetIn2 A m n)=>x ty. elim: ty A m n e=>//{Γ B x}.
+  { move=>Γ1 Γ2 Γ A B C m n s r t k x leq key mrg tym _ tyC _ tyn _
+      A0 m0 n0[e1 e2 e3]; subst.
+    apply: sim_refl. }.
+  { move=>Γ A B m s k tym ihm tyB _ A0 m0 n e; subst.
+    have eq':=ihm _ _ _ erefl.
+    apply: sim_transL... }
+Qed.
+
+Lemma clc_main_uniq Γ B :
+  Γ ⊢ Main : B -> sim (Sort L) B.
+Proof with eauto.
+  move e:(Main)=>x ty. elim: ty e=>//{Γ x B}.
+  move=>Γ A B m s eq tym ih tyB _ e; subst.
+  have eq':=ih erefl.
+  apply: sim_transL...
+Qed.
+
+Lemma clc_proto_uniq Γ B :
+  Γ ⊢ Proto : B -> sim (Sort U) B.
+Proof with eauto.
+  move e:(Proto)=>x ty. elim: ty e=>//{Γ x B}.
+  move=>Γ A B m s eq tym ih tyB _ e; subst.
+  have eq':=ih erefl.
+  apply: sim_transL...
+Qed.
+
+Lemma clc_stop_uniq Γ B r :
+  Γ ⊢ Stop r : B -> sim (Proto) B.
+Proof with eauto.  
+  move e:(Stop r)=>x ty. elim: ty r e=>//{Γ x B}.
+  move=>Γ A B m s eq tym ih tyB _ r e; subst.
+  have eq':=ih _ erefl.
+  apply: sim_transL...
+Qed.
+
+Lemma clc_act_uniq Γ A B C s r :
+  Γ ⊢ Act r A B s : C -> sim (Proto) C.
+Proof with eauto.  
+  move e:(Act r A B s)=>x ty. elim: ty A B s r e=>//{Γ x C}.
+  move=>Γ A B m s eq tym ihm tyB _ A0 B0 s0 r e; subst.
+  have eq':=ihm _ _ _ _ erefl.
+  apply: sim_transL...
+Qed.
+
+Lemma clc_ch_uniq Γ A B r :
+  Γ ⊢ Ch r A : B -> sim (Sort L) B.
+Proof with eauto.
+  move e:(Ch r A)=>x ty. elim: ty r A e=>//{Γ x B}.
+  move=>Γ A B m s eq tym ihm tyB _ r A0 e; subst.
+  have eq':=ihm _ _ erefl.
+  apply: sim_transL...
+Qed.
+
+Lemma clc_fork_uniq Γ m n A C r :
+  Γ ⊢ Fork m n : C -> sim (Sigma (Ch (~~r) A) Main L L L) C.
+Proof with eauto.
+  move e:(Fork m n)=>x ty. elim: ty A m n r e=>//{Γ x C}.
+  { move=>Γ1 Γ2 r1 r2 Γ m n A B t mrg d tyA _ tym _ tyn _
+      A0 B0 m0 r[e1 e2]; subst.
+    econstructor. eauto.
+    econstructor. eauto. }
+  { move=>Γ A B m s eq tym ihm tyB _ A0 B0 m0 r e; subst.
+    have eq':=ihm _ _ _ _ erefl.
+    apply: sim_transL... }
+Qed.
+
+Lemma clc_recv_uniq Γ m A B C s r :
+  Γ ⊢ Recv m : C -> sim (Sigma A (Ch r B) s L L) C.
+Proof with eauto.
+  move e:(Recv m)=>x ty. elim: ty A B m s r e=>//{Γ x C}.
+  { move=>*.
+    econstructor. eauto.
+    econstructor. eauto. }
+  { move=>Γ A B m s eq tym ihm tyB _ A0 B0 m0 s0 r e; subst.
+    have eq':=ihm A0 B0 _ s0 r erefl.
+    apply: sim_transL... }
+Qed.
+
+Lemma clc_send_uniq Γ m A B C s r1 r2 :
+  Γ ⊢ Send m : C ->
+  (forall C, Γ ⊢ m : C -> sim (Ch r1 (Act r2 A B s)) C) ->
+  sim (Pi A (Ch r1 B) s L) C.
+Proof with eauto.
+  move e:(Send m)=>x ty. elim: ty A B m s r1 r2 e=>//{Γ x C}.
+  { move=>Γ r1 r2 A B m s xor tym _ A0 B0 m0 s0 r0 r3[e]h; subst.
+    
+  }
+
+  ihm : ∀ (Γ2 G1 G2 Γ0 : context term) (B0 : term),
+          Γ2 ⊢ m : B0 → Γ ∘ G1 => Γ0 → Γ2 ∘ G2 => Γ0 → sim (Ch r1 (Act r2 A B s)) B0
+  Γ2, G1, G2, Γ0 : context term
+  B0 : term
+  ty : Γ2 ⊢ Send m : B0
+  mrg1 : Γ ∘ G1 => Γ0
+  mrg2 : Γ2 ∘ G2 => Γ0
+  ============================
+  sim (Pi A (Ch r1 B) s L) B0
 
 Lemma clc_uniq Γ1 Γ2 G1 G2 Γ m A B :
-  Γ1 ⊢ m : A -> Γ2 ⊢ m : B ->
-  Γ1 ∘ G1 => Γ -> Γ2 ∘ G2 => Γ -> A === B.
+  Γ1 ⊢ m : A -> Γ2 ⊢ m : B -> Γ1 ∘ G1 => Γ -> Γ2 ∘ G2 => Γ -> sim A B.
 Proof with eauto.
   move=>ty. elim: ty Γ2 G1 G2 Γ B=>{Γ1 m A}.
-  { move=>*. apply: clc_sort_uniq... }
-  { move=>*. apply: clc_pi_uniq... }
+  { move=>Γ s k Γ2 G1 G2 Γ0 B tyS mrg1 mrg2.
+    apply: clc_sort_uniq... }
+  { move=>Γ A B s r t k tyA ihA tyB ihB Γ1 G1 G2 Γ0 B0 tyP mrg3 mrg4.
+    apply: clc_pi_uniq... }
   { move=>Γ x A s hs Γ2 G1 G2 Γ0 B tyV mrg1 mrg2.
-    have[X[t[hsx eq]]]:=var_inv tyV.
-    have[-> _//]:=clc_has_subset hs hsx mrg1 mrg2. }
+    have[X[v[hsx eq]]]:=var_inv tyV.
+    have[-> _//]:=clc_has_subset hs hsx mrg1 mrg2.
+    econstructor... }
   { move=>Γ A B m s t k tyP ihP tym ihm Γ2 G1 G2 Γ0 B0 tyL mrg1 mrg2.
-    apply: clc_lam_uniq...
+    apply:clc_lam_uniq...
     move=>C tym'.
     destruct s.
     have{}mrg1: A :U Γ ∘ A :U G1 => A :U Γ0 by constructor.
@@ -227,23 +464,53 @@ Proof with eauto.
     apply: clc_sigma_uniq... }
   { move=>Γ1 Γ2 Γ A B m n s r t k1 k2 mrg tyS ihS tym ihm tyn ihn Γ0 G1 G2 Γ3 B0 tyP mrg1 mrg2.
     apply: clc_pair_uniq...
-    admit.
-    admit.
-    intros.
-    split.
+    move=>Γ4 Γ5 G0 G3 X Y tyx mrgx tyy mrgy. split.
     have[D1[mrg3 mrg4]]:=merge_splitR mrg1 mrg.
-    have[D2[mrg5 mrg6]]:=merge_splitR mrg2 H0.
-    apply: ihm.
-    exact: H.
-    exact: mrg4.
-    exact: mrg6.
+    have[D2[mrg5 mrg6]]:=merge_splitR mrg2 mrgx.
+    apply: ihm. exact: tyx. exact: mrg4. exact: mrg6.
     have[D1[mrg3 mrg4]]:=merge_splitR mrg1 (merge_sym mrg).
-    have[D2[mrg5 mrg6]]:=merge_splitR mrg2 (merge_sym H2).
-    apply: ihn.
-    exact: H1.
-    exact: mrg4.
-    exact: mrg6.
-
-
+    have[D2[mrg5 mrg6]]:=merge_splitR mrg2 (merge_sym mrgy).
+    apply: ihn. exact: tyy. exact: mrg4. exact: mrg6. }
+  { move=>Γ1 Γ2 Γ m n1 n2 A s t k mrg tym ihm tyA ihA tyn1 ihn1 tyn2 ihn2
+      Γ0 G1 G2 Γ3 B tyC mrg1 mrg2.
+    apply: clc_case_uniq... }
+  { move=>Γ1 Γ2 Γ m n A s t k mrg tym ihm tyA ihA tyn ihn
+      Γ0 G1 G2 Γ3 B tyL mrg1 mrg2.
+    apply: clc_letin1_uniq... }
+  { move=>Γ1 Γ2 Γ A B C m n s r t k x leq key mrg tym _ tyC _ tyn _
+      Γ0 G1 G2 Γ3 B0 tyL mrg1 mrg2.
+    apply: clc_letin2_uniq... }
+  { move=>Γ k Γ1 G1 G2 Γ0 B tyM mrg1 mrg2.
+    apply: clc_main_uniq... }
+  { move=>Γ k Γ2 G1 G2 Γ0 B tyP mrg1 mrg2.
+    apply: clc_proto_uniq... }
+  { move=>Γ r k Γ2 G1 G2 Γ0 B tyS mrg1 mrg2.
+    apply: clc_stop_uniq... }
+  { move=>Γ r A B s k tyA ihA tyB ihB Γ2 G1 G2 Γ0 B0 ty mrg1 mrg2.
+    apply: clc_act_uniq... }
+  { move=>Γ r A k tyA ihA Γ2 G1 G2 Γ0 B tyC mrg1 mrg2.
+    apply: clc_ch_uniq... }
+  { move=>Γ1 Γ2 r1 r2 Γ m n A B t mrg d tyA ihA tym ihm tyn ihn
+      Γ0 G1 G2 Γ3 B0 tyF mrg1 mrg2; subst.
+    apply: clc_fork_uniq... }
+  { move=>Γ r1 r2 A B m s xor tym ihm Γ2 G1 G2 Γ0 B0 ty mrg1 mrg2.
+    apply: clc_recv_uniq... }
+  { move=>Γ r1 r2 A B m s xor tym ihm Γ2 G1 G2 Γ0 B0 ty mrg1 mrg2.
     
   }
+  admit.
+  admit.
+  admit.
+  admit.
+  admit.
+  admit.
+  admit.
+  admit.
+  admit.
+  admit.
+  admit.
+  admit.
+  intros.
+  have eq':=H1 _ _ _ _ _ H4 H5 H6.
+  apply: sim_transR...
+  apply: conv_sym...
