coq/cclc3/clc_soundness.v
@@ -76,7 +76,7 @@ Proof with eauto using clc_type, step, ok, merge_re_id.
       apply: clc_app...
       exact: tyB. }
     { simpl in tyB. rewrite<-re_invo in tyB.
-      have {}tyB := substitutionN tyB tyn.
+      have {}tyB := substitutionN n tyB.
       apply: clc_conv.
       apply: conv_beta.
       apply: conv1i...
@@ -153,7 +153,7 @@ Proof with eauto using clc_type, step, ok, merge_re_id.
     rewrite e5 e2 (pure_re k1) e1.
     apply:merge_re_id.
     have:=substitution tyB k1 mrg1 tym'. asimpl...
-    have:=substitutionN tyB tym'. 
+    have:=substitutionN m' tyB.
     rewrite e5. rewrite<-e2... }
   { move:(ihn _ o2 H3)=>{ihm ihS ihn}tyn'.
     apply:clc_pair... }
@@ -173,7 +173,55 @@ Proof with eauto using clc_type, step, ok, merge_re_id.
     apply: re_ok... }
   have[_[e1 e2]]:=merge_re_re mrg.
   inv st.
-  { have{}ihm:=ihm _ H3.
+  { have{}ihA:=ihA _ H4.
+    destruct s; simpl in ihA; simpl in tyA.
+    have mrg':[Γ2] ∘ Γ1 => [Γ].
+    { replace Γ1 with [Γ1].
+      apply: merge_re3. apply: merge_sym...
+      rewrite<-pure_re... }
+    have tyL: [Γ1] ⊢ Left : Either.
+    { constructor. apply: re_pure. }
+    have tyR: [Γ1] ⊢ Right : Either.
+    { constructor. apply: re_pure. }
+    have tymA:=substitution tyA k mrg' tym.
+    have tymA':=substitution ihA k mrg' tym.
+    have tyAL:=substitution ihA (re_pure _) (merge_re3 (merge_sym mrg)) tyL.
+    have tyAR:=substitution ihA (re_pure _) (merge_re3 (merge_sym mrg)) tyR.
+    apply: clc_conv.
+    apply: conv_subst.
+    apply: conv1i...
+    apply: clc_case...
+    apply: clc_conv.
+    apply: conv_subst.
+    apply: conv1...
+    eauto.
+    rewrite e2...
+    apply: clc_conv.
+    apply: conv_subst.
+    apply: conv1...
+    eauto.
+    rewrite e2...
+    eauto.
+    have tymA:=substitutionN m tyA.
+    have tymA':=substitutionN m ihA.
+    have tyAL:=substitutionN Left ihA.
+    have tyAR:=substitutionN Right ihA.
+    apply: clc_conv.
+    apply: conv_subst.
+    apply: conv1i...
+    apply: clc_case...
+    apply: clc_conv.
+    apply: conv_subst.
+    apply: conv1...
+    eauto.
+    eauto.
+    apply: clc_conv.
+    apply: conv_subst.
+    apply: conv1...
+    eauto.
+    eauto.
+    rewrite<-e2... }
+  { have{}ihm:=ihm _ H4.
     destruct s; simpl in tyA.
     have mrg':[Γ2] ∘ Γ1 => [Γ].
     { replace Γ1 with [Γ1].
@@ -185,28 +233,88 @@ Proof with eauto using clc_type, step, ok, merge_re_id.
     apply: conv1i...
     apply: clc_case...
     apply: tymA.
-    have tymA:=substitutionN tyA tym.
+    have tymA:=substitutionN m tyA.
     apply: clc_conv.
     apply: conv_beta.
     apply: conv1i...
     apply: clc_case...
     rewrite<-e2... }
-  { have{}ihn1:=ihn1 _ H3.
+  { have{}ihn1:=ihn1 _ H4.
     apply: clc_case... }
-  { have{}ihn2:=ihn2 _ H3.
+  { have{}ihn2:=ihn2 _ H4.
     apply: clc_case... }
   { have k1:=left_inv tym.
     have->//:=merge_pureL mrg k1. }
   { have k1:=right_inv tym.
     have->//:=merge_pureL mrg k1. }
-  move=>Γ1 Γ2 Γ m n A mrg tym ihm tyn ihn n0 o st.
+  move=>Γ1 Γ2 Γ m n A s t k mrg tym ihm tyA ihA tyn ihn n0 o st.
   move:(merge_context_ok_inv mrg o)=>[o1 o2]. inv st.
-  { move:(ihm _ o1 H2)=>tym'.
+  { have[e1[e2 e3]]:=merge_re_re mrg.
+    have tyI:[Γ1] ⊢ It : Unit.
+    { constructor. apply: re_pure. }
+    destruct s; simpl in ihA; simpl in tyA.
+    have oA:ok (Unit :U [Γ2]).
+    { constructor. apply: re_ok...
+      constructor. apply: re_pure... }
+    have tyA':=ihA _ oA H3.
+    have mrg':[Γ2] ∘ Γ1 => [Γ].
+    { replace Γ1 with [Γ1].
+      apply: merge_re3. apply: merge_sym...
+      rewrite<-pure_re... }
+    have tymA:=substitution tyA k mrg' tym.
+    have tymA':=substitution tyA' k mrg' tym.
+    have tyIA:=substitution tyA' (re_pure _) (merge_re3 (merge_sym mrg)) tyI.
+    apply: clc_conv.
+    apply: conv_subst.
+    apply: conv1i...
+    apply: clc_letin1...
+    apply: clc_conv.
+    apply: conv_subst.
+    apply: conv1...
+    eauto.
+    rewrite e3...
+    eauto.
+    have tyA':=ihA _ (n_ok (re_ok o2)) H3.
+    have tymA:=substitutionN m tyA.
+    have tymA':=substitutionN m tyA'.
+    have tyIA:=substitutionN It tyA'.
+    apply: clc_conv.
+    apply: conv_subst.
+    apply: conv1i...
+    apply: clc_letin1...
+    apply: clc_conv.
+    apply: conv_subst.
+    apply: conv1...
+    eauto.
+    eauto.
+    rewrite<-e3... }
+  { move:(ihm _ o1 H3)=>tym'.
+    have[e1[e2 e3]]:=merge_re_re mrg.
+    have tyI:[Γ1] ⊢ It : Unit.
+    { constructor. apply: re_pure. }
+    destruct s; simpl in tyA.
+    have mrg':[Γ2] ∘ Γ1 => [Γ].
+    { replace Γ1 with [Γ1].
+      apply: merge_re3. apply: merge_sym...
+      rewrite<-pure_re... }
+    have tymA:=substitution tyA k mrg' tym.
+    have tymA':=substitution tyA k mrg' tym'.
+    apply: clc_conv.
+    apply: conv_beta.
+    apply: conv1i...
+    apply: clc_letin1...
+    eauto.
+    have tymA:=substitutionN m tyA.
+    have tymA':=substitutionN m' tyA.
+    apply: clc_conv.
+    apply: conv_beta.
+    apply: conv1i...
+    apply: clc_letin1...
+    rewrite<-e3... }
+  { move:(ihn _ o2 H3)=>tyn'.
     apply: clc_letin1... }
-  { move:(ihn _ o2 H2)=>tyn'.
-    apply: clc_letin1... }
-  { move:(it_inv tym)=>k.
-    by rewrite (merge_pureL mrg k). }
+  { move:(it_inv tym)=>pk.
+    by rewrite (merge_pureL mrg pk). }
   move=>Γ1 Γ2 Γ A B C m n s r t k x leq key mrg
     tym ihm tyC ihC tyn ihn n0 o st.
   move:(merge_context_ok_inv mrg o)=>[o1 o2]. 
@@ -215,7 +323,133 @@ Proof with eauto using clc_type, step, ok, merge_re_id.
   move:(merge_re_re mrg)=>[e0[e1 e2]].
   move:(merge_re_re mrg0)=>[e3[e4 e5]].
   inv st.
-  { move:(ihm _ o1 H2)=>tym'.
+  { destruct k; simpl in tyC; simpl in ihC. inv leq.
+    have[D1[D2[leq _]]]:=sigma_inv tyS. inv leq.
+    destruct s; destruct r; inv H0.
+    have[k1 k2]:=merge_pure_inv mrg0 (re_pure _).
+    have[e6 e7]:=merge_pure_eq mrg0 k1 k2.
+    have{}tyS:[Γ2] ⊢ Sigma A B U U U : Sort U.
+    { rewrite<-e0.
+      apply: clc_sigma...
+      constructor.
+      apply: re_pure.
+      rewrite<-e6...
+      rewrite<-e7... }
+    have oS:ok (Sigma A B U U U :U [Γ2]).
+    { constructor. apply: re_ok...
+      rewrite<-re_invo... }
+    have mrg':[Γ2] ∘ Γ1 => [Γ].
+    { replace Γ1 with [Γ1].
+      apply: merge_re3. apply: merge_sym...
+      rewrite<-pure_re... }
+    have tyA':=ihC _ oS H3.
+    have tymC:=substitution tyC key mrg' tym.
+    have tyP: B :U A :U [Γ2] ⊢ Pair (Var 1) (Var 0) U : (Sigma A B U U U).[ren (+2)].
+    { have k0: B :U A :U [Γ2] |> U.
+      { repeat constructor. apply: re_pure. }
+      have mrg2:B :U A :U [Γ2] ∘ B :U A :U [Γ2] => B :U A :U [Γ2].
+      { constructor.
+        constructor.
+        apply: merge_re_id. }
+      apply: clc_pair.
+      apply: k0.
+      apply: k0.
+      apply: mrg2.
+      simpl. rewrite<-re_invo.
+      have{}tyS:=weakeningU A tyS.
+      have{}tyS:=weakeningU B tyS.
+      asimpl in tyS.
+      asimpl...
+      apply: clc_var.
+      replace A.[ren (+2)] with A.[ren (+1)].[ren (+1)] by autosubst.
+      econstructor.
+      econstructor.
+      apply: re_pure.
+      apply: clc_var.
+      asimpl.
+      econstructor.
+      constructor.
+      apply: re_pure. }
+    have tyAx:B :U A :U [Γ2] ⊢ A'.[Pair (Var 1) (Var 0) U .: ren (+2)] : Sort x.
+    { have tyAx: (Sigma A B U U U).[ren (+2)] :U B :U A :U [Γ2] ⊢
+                   A'.[ren (upren (+2))] : (Sort x).[ren (upren (+2))].
+      { apply: rename_ok.
+        apply: tyA'.
+        constructor.
+        constructor.
+        constructor.
+        apply: agree_ren_refl. }
+      replace (Sort x) with (Sort x).[up (ren (+2))].[(Pair (Var 1) (Var 0) U)/] by autosubst.
+      replace A'.[Pair (Var 1) (Var 0) U .: ren (+2)]
+         with A'.[up (ren (+2))].[(Pair (Var 1) (Var 0) U)/] by autosubst.
+      apply: esubstitution.
+      asimpl. asimpl in tyAx.
+      apply: tyAx.
+      constructor.
+      apply: agree_subst_refl.
+      asimpl.
+      rewrite<-re_invo.
+      asimpl in tyP... }
+    apply: clc_conv.
+    apply: conv_subst.
+    apply: conv1i...
+    apply: clc_letin2.
+    constructor.
+    apply: key.
+    apply: mrg.
+    all: eauto.
+    apply: clc_conv.
+    apply: conv_subst.
+    apply: conv1...
+    eauto.
+    eauto.
+    have oS:ok (_: [Γ2]).
+    { constructor. apply: re_ok... }
+    have tyA':=ihC _ oS H3.
+    have tymC:=substitutionN m tyC.
+    have tyAx: _: [B :{r} A :{s} Γ2] ⊢ A'.[ren (upren (+2))] : (Sort x).[ren (upren (+2))].
+    { destruct r; destruct s.
+      apply: rename_ok.
+      apply: tyA'.
+      constructor; simpl.
+      constructor.
+      constructor.
+      apply: agree_ren_refl.
+      apply: rename_ok.
+      apply: tyA'.
+      constructor; simpl.
+      constructor.
+      constructor.
+      apply: agree_ren_refl.
+      apply: rename_ok.
+      apply: tyA'.
+      constructor; simpl.
+      constructor.
+      constructor.
+      apply: agree_ren_refl.
+      apply: rename_ok.
+      apply: tyA'.
+      constructor; simpl.
+      constructor.
+      constructor.
+      apply: agree_ren_refl. }
+    have tyP:=substitutionN (Pair (Var 1) (Var 0) t) tyAx.
+    apply: clc_conv.
+    apply: conv_subst.
+    apply: conv1i...
+    apply: clc_letin2.
+    apply: leq.
+    apply: key.
+    apply: mrg.
+    all: eauto.
+    apply: clc_conv.
+    apply: conv_subst.
+    apply: conv1...
+    all: eauto.
+    asimpl in tyP.
+    asimpl...
+    rewrite<-e2... }
+  { move:(ihm _ o1 H3)=>tym'.
     apply: clc_conv.
     apply: conv_beta.
     apply: conv1i...
@@ -226,7 +460,7 @@ Proof with eauto using clc_type, step, ok, merge_re_id.
     apply:merge_re_id. inv leq.
     have:=substitution tyC key mrg1 tym.
     asimpl...
-    have:=substitutionN tyC tym.
+    have:=substitutionN m tyC.
     asimpl. by rewrite e2. }
   { rewrite<-re_invo in e4.
     rewrite<-re_invo in e5.
@@ -236,7 +470,7 @@ Proof with eauto using clc_type, step, ok, merge_re_id.
     econstructor...
     rewrite<-e0. rewrite<-e4. rewrite<-pure_re...
     move:tyB; destruct s=>//=; rewrite e5 e0...
-    move:(ihn _ oAB H2)=>tyn'.
+    move:(ihn _ oAB H3)=>tyn'.
     apply: clc_letin2... }
   { rewrite<-re_invo in e4.
     rewrite<-re_invo in e5.
